README.md
@@ -61,12 +61,10 @@ lake exe export_contract
 
 ### In a machine terminal
 
-After you get a copy of this repo in your own GitHub account,
-open a machine terminal in `Repos` or where you want the project:
+Open a machine terminal where you want the project:
 
 ```shell
-# Replace username with YOUR GitHub username.
-git clone https://github.com/username/se-formal-contract
+git clone https://github.com/structural-explainability/se-formal-contract
 
 cd se-formal-contract
 code .
